theory/x64DecodeProof.thy
@@ -2,8 +2,10 @@ theory x64DecodeProof
 imports
   Main
   rBPFCommType rBPFSyntax
-  x64Assembler x64Disassembler
+  x64Assembler x64Disassembler BitsOpMore2
 begin
+
+declare if_split_asm [split]
 
 lemma [simp]: "l @ [a] = l_bin \<Longrightarrow> l_bin!(length l) = a" by fastforce
 lemma [simp]: "l @ [a, b] = l_bin \<Longrightarrow> l_bin!(length l) = a" by fastforce  
@@ -67,6 +69,22 @@ lemma [simp]: "l @ [a, b, c] = l_bin \<Longrightarrow> length l_bin - length l =
 lemma [simp]: "l @ [a, b, c, d] = l_bin \<Longrightarrow> length l_bin - length l = 4" by fastforce
 lemma [simp]: "l @ [a, b, c, d, e] = l_bin \<Longrightarrow> length l_bin - length l = 5" by fastforce
 
+lemma [simp]: "length l1 = 8 \<Longrightarrow> list_in_list l1 pc l \<Longrightarrow>
+[l ! pc, l ! (pc + 1), l ! (pc + 2), l ! (pc + 3), l ! (pc + 4), l ! (pc + 5), 
+  l ! (pc + 6), l ! (pc + 7)] = l1"
+  apply (cases "l1", simp)
+  subgoal for a1 l1 apply (cases "l1", simp)
+  subgoal for a2 l2 apply (cases "l2", simp)
+  subgoal for a3 l3 apply (cases "l3", simp)
+  subgoal for a4 l4 apply (cases "l4", simp)
+  subgoal for a5 l5 apply (cases "l5", simp)
+  subgoal for a6 l6 apply (cases "l6", simp)
+  subgoal for a7 l7 apply (cases "l7", simp)
+  subgoal for a8 l8 apply (cases "l8", simp)
+    apply (simp add: eval_nat_numeral(3) numeral_Bit0)
+  subgoal for a9 l9 apply (cases "l9", simp)
+    subgoal for a10 l10 apply (cases "l10", simp) 
+      sorry
 
 lemma x64_encode_decode_consistency:
   "list_in_list l_bin pc l \<Longrightarrow> Some l_bin = x64_encode ins \<Longrightarrow> x64_decode pc l = Some (length l_bin, ins)"
@@ -75,7 +93,7 @@ lemma x64_encode_decode_consistency:
   subgoal for dst src
   \<comment> \<open> Pmovl_rr \<close> 
     apply (unfold Let_def)
-    apply (cases "construct_rex_to_u8 False (and (u8_of_ireg src) 8 \<noteq> 0) False (and (u8_of_ireg dst) 8 \<noteq> 0) = 0"; simp_all add: construct_rex_to_u8_def construct_modsib_to_u8_def; erule conjE)
+    apply (cases "construct_rex_to_u8 False (and (u8_of_ireg src) 8 \<noteq> 0) False (and (u8_of_ireg dst) 8 \<noteq> 0) = 64"; simp_all add: construct_rex_to_u8_def construct_modsib_to_u8_def; erule conjE)
     subgoal by (cases src; cases dst; auto simp add: x64_decode_def bitfield_insert_u8_def Let_def ireg_of_u8_def)
     subgoal by (cases src; cases dst; auto simp add: x64_decode_def bitfield_insert_u8_def Let_def ireg_of_u8_def)
     done
@@ -86,8 +104,30 @@ lemma x64_encode_decode_consistency:
     subgoal by (cases src; cases dst; auto simp add: x64_decode_def bitfield_insert_u8_def Let_def ireg_of_u8_def)
     done
 
+  subgoal for dst imm
+  \<comment> \<open> Pmovl_ri  
+    apply (unfold Let_def)
+    apply (cases "construct_rex_to_u8 False False False (and (u8_of_ireg dst) 8 \<noteq> 0) = 0"; simp_all add:construct_rex_to_u8_def construct_modsib_to_u8_def; erule conjE )
+    subgoal 
+      apply (cases dst;cases imm; auto simp add: x64_decode_def bitfield_insert_u8_def Let_def ireg_of_u8_def )\<close>
+    sorry
+
+  subgoal for dst imm
+ \<comment> \<open> Pmovq_ri
+    apply (cases dst; simp add: construct_rex_to_u8_def bitfield_insert_u8_def x64_decode_def Let_def ireg_of_u8_def)
+
+    apply (cases "l ! pc = 144", simp)
+    subgoal by (cases dst; simp)
+
+    apply (simp add: x64_decode_def Let_def construct_rex_to_u8_def bitfield_insert_u8_def construct_modsib_to_u8_def)
+    apply (cases "construct_rex_to_u8 True False False (and (u8_of_ireg dst) 8 \<noteq> 0) = 0"; simp_all add:construct_rex_to_u8_def construct_modsib_to_u8_def; erule conjE )
+    subgoal 
+    subgoal 
+      apply (unfold x64_decode_def bitfield_insert_u8_def Let_def ireg_of_u8_def u8_list_of_u64_def )\<close>
+    sorry
+      
   subgoal for src dst chunk
-  \<comment> \<open> Pmov_rm \<close> 
+  \<comment> \<open> Pmov_rm 
     apply (cases dst, simp)
     subgoal for rd rs ro
       apply (cases rd, simp_all)
@@ -95,9 +135,33 @@ lemma x64_encode_decode_consistency:
         apply (cases rs, simp_all)
         apply (cases "rd1 = ireg.R11 \<and> ro = 0", simp_all add: Let_def)
         apply (unfold Let_def construct_rex_to_u8_def construct_modsib_to_u8_def)
-        apply (cases chunk; cases src; auto simp add: x64_decode_def bitfield_insert_u8_def Let_def ireg_of_u8_def)
-        done
-      done
+        apply (cases chunk; cases src; auto simp add: x64_decode_def bitfield_insert_u8_def Let_def ireg_of_u8_def)\<close> 
+    sorry
+
+  subgoal for src dst chunk
+    \<comment> \<open> Pmov_mr \<close> 
+    sorry
+
+  subgoal for src dst chunk
+    \<comment> \<open> Pmov_mi \<close> 
+    sorry
+
+  subgoal for src dst
+    \<comment> \<open> Pxchg_rr \<close> 
+    apply (unfold Let_def construct_rex_to_u8_def construct_modsib_to_u8_def; erule conjE; erule conjE)
+    subgoal by (cases src; cases dst; auto simp add: x64_decode_def bitfield_insert_u8_def Let_def ireg_of_u8_def)
+    done
+
+  subgoal for src dst
+    \<comment> \<open> Pmovsq_rr \<close> 
+    apply (unfold Let_def construct_rex_to_u8_def construct_modsib_to_u8_def; erule conjE; erule conjE)
+    subgoal by (cases src; cases dst; auto simp add: x64_decode_def bitfield_insert_u8_def Let_def ireg_of_u8_def)
+    done
+
+  subgoal for dst
+    \<comment> \<open> Pnegl_rr \<close> 
+    apply (unfold Let_def construct_rex_to_u8_def construct_modsib_to_u8_def; erule conjE; erule conjE)
+    subgoal by (cases dst; auto simp add: x64_decode_def bitfield_insert_u8_def Let_def ireg_of_u8_def)
     done
 
  \<comment> \<open> 
